

Homework 4 Solutions

1

Problem 4-1

$$\psi_k[n] = e^{j k (2\pi/N) n}$$

$$k = 0, 1, \dots, N-1$$

$$\sum_{n=0}^{N-1} \psi_k[n] \psi_m^*[n] = \sum_{n=0}^{N-1} e^{j k \frac{2\pi}{N} n} e^{-j m \frac{2\pi}{N} n}$$

$$= \sum_{n=0}^{N-1} e^{j \frac{2\pi}{N} n (k-m)}$$

$$\text{Let } \alpha = e^{j \frac{2\pi}{N} (k-m)}$$

$$\Rightarrow \sum_{n=0}^{N-1} \alpha^n = \begin{cases} \frac{1-\alpha^N}{1-\alpha} & \alpha \neq 1 \\ N & \alpha = 1 \end{cases}$$

$$\text{So, } \sum_{n=0}^{N-1} e^{j \frac{2\pi}{N} n (k-m)} = \begin{cases} \frac{1 - e^{j \frac{2\pi}{N} (k-m) N}}{1 - e^{j \frac{2\pi}{N} (k-m)}} & k \neq m \\ N & k = m \end{cases}$$

$$\text{notice that } e^{j \frac{2\pi}{N} (k-m) N} = e^{j 2\pi (k-m)} = e^{j 2\pi k} e^{-j 2\pi m} = 1$$

Therefore,

$$\sum_{n=0}^{N-1} \psi_k[n] \psi_m^*[n] = \begin{cases} 0 & k \neq m \\ N & k = m \end{cases}$$

Problem 4-2

$$\begin{aligned} \text{DTFT} \{ e^{j\omega_0 n} x[n] \} &= \sum_{n=-\infty}^{\infty} e^{j\omega_0 n} x[n] e^{-j\omega n} \\ &= \sum_{n=-\infty}^{\infty} x[n] e^{-j(\omega - \omega_0)n} = X(e^{j(\omega - \omega_0)}) \end{aligned}$$

Problem 4-3

$$\begin{aligned} x(t) &= \frac{1}{2\pi} \int_{-\infty}^{\infty} X(j\Omega) e^{+j\Omega t} d\Omega \\ &= \frac{1}{2\pi} \int_{-\infty}^{\infty} 2\pi \delta(\Omega - \Omega_0) e^{+j\Omega t} d\Omega \\ &= \int_{-\infty}^{\infty} \delta(\Omega - \Omega_0) e^{+j\Omega t} d\Omega = e^{j\Omega_0 t} \end{aligned}$$

Problem 4-4

$$n x[n] \xleftrightarrow{\text{DTFT}} j \frac{dX(e^{j\omega})}{d\omega}$$

$$X(e^{j\omega}) = \sum_{n=-\infty}^{\infty} x[n] e^{-j\omega n}$$

$$\frac{dX(e^{j\omega})}{d\omega} = \frac{d}{d\omega} \sum_{n=-\infty}^{\infty} x[n] e^{-j\omega n} = \sum_{n=-\infty}^{\infty} x[n] \frac{d}{d\omega} e^{-j\omega n}$$

$$= -j \sum_{n=-\infty}^{\infty} n x[n] e^{-j\omega n}$$

Multiply both sides by j

$$j \frac{dX(e^{j\omega})}{d\omega} = \sum_{n=-\infty}^{\infty} n x[n] e^{-j\omega n} //$$

Problem 4-5

$$\text{DTFT}\{x[n-n_0]\} = \sum_{n=-\infty}^{\infty} x[n-n_0] e^{-j\omega n}$$

Let $m = n - n_0$

$$\Rightarrow \sum_{m=-\infty}^{\infty} x[m] e^{-j\omega(m+n_0)}$$

$$= e^{-j\omega n_0} \sum_{m=-\infty}^{\infty} x[m] e^{-j\omega m}$$

$$= e^{-j\omega n_0} X(e^{j\omega})$$

so,

$$x[n-n_0] \longleftrightarrow e^{-j\omega n_0} X(e^{j\omega})$$

Problem 4-6

see matlab code for Hw 4

Problem 4-7

The freq. Resp. is the DTFT of the impulse response, so

$$H_1(e^{j\omega}) = \frac{1}{2} + \frac{1}{2} e^{-j\omega} = e^{-j\frac{\omega}{2}} \left(\frac{e^{j\frac{\omega}{2}} + e^{-j\frac{\omega}{2}}}{2} \right)$$

$$= e^{-j\frac{\omega}{2}} \cos(\omega/2)$$

$$|H_1(e^{j\omega})| = |\cos(\omega/2)| = \cos^2(\omega/2)$$

Also,

$$H_2(e^{j\omega}) = \frac{1}{2} - \frac{1}{2} e^{-j\omega} = j e^{-j\frac{\omega}{2}} \left(\frac{e^{j\frac{\omega}{2}} - e^{-j\frac{\omega}{2}}}{2j} \right) = j e^{-j\frac{\omega}{2}} \sin(\omega/2)$$

$$|H_2(e^{j\omega})| = |\sin(\omega/2)| = \sin^2(\omega/2)$$

see matlab plots for Hw 4